unity/code/syntax.lean
@@ -20,35 +20,35 @@ parameters {σ}
 
 inductive code : pred → pred → Type
   | skip {} : ∀ p, code p p
-  | action : ∀ p q, lbl → code p q
+  | action : ∀ p q, set lbl → lbl → code p q
   | seq : ∀ {p q r}, code p q → code q r → code p r
-  | if_then_else : ∀ p {pa pb q}, pred → code pa q → code pb q → code p q
-  | while : ∀ {p inv} q, pred → code p inv → code inv q
+  | if_then_else : ∀ p {pa pb q}, set lbl → pred → code pa q → code pb q → code p q
+  | while : ∀ {p inv} q, set lbl → pred → code p inv → code inv q
 
 parameters {σ lbl}
 
 @[pattern,reducible]
-def if_then_else : ∀ p {pa pb q}, pred → code pa q → code pb q → code p q :=
+def if_then_else : ∀ p {pa pb q}, set lbl → pred → code pa q → code pb q → code p q :=
 code.if_then_else
 
 @[pattern,reducible]
-def while : ∀ {p inv} q, pred → code p inv → code inv q :=
+def while : ∀ {p inv} q, set lbl → pred → code p inv → code inv q :=
 @code.while
 
 inductive current : ∀ {p q}, code p q → Type
-  | action : ∀ p q l, current (code.action p q l)
+  | action : ∀ p q s l, current (code.action p q s l)
   | seq_left : ∀ p q r (c₀ : code p q) (c₁ : code q r), current c₀ → current (code.seq c₀ c₁)
   | seq_right : ∀ p q r (c₀ : code p q) (c₁ : code q r), current c₁ → current (code.seq c₀ c₁)
-  | if_then_else_cond  : ∀ p t pa pb q (c₀ : code pa q) (c₁ : code pb q),
-         current (code.if_then_else p t c₀ c₁)
-  | if_then_else_left  : ∀ p t pa pb q (c₀ : code pa q) (c₁ : code pb q),
-         current c₀ → current (code.if_then_else p t c₀ c₁)
-  | if_then_else_right : ∀ p t pa pb q (c₀ : code pa q) (c₁ : code pb q),
-         current c₁ → current (code.if_then_else p t c₀ c₁)
-  | while_cond : ∀ p inv q w (c : code p inv),
-         current (code.while q w c)
-  | while_body : ∀ p inv q w (c : code p inv),
-         current c → current (code.while q w c)
+  | if_then_else_cond  : ∀ p t pa pb q s (c₀ : code pa q) (c₁ : code pb q),
+         current (code.if_then_else p s t c₀ c₁)
+  | if_then_else_left  : ∀ p t pa pb q s (c₀ : code pa q) (c₁ : code pb q),
+         current c₀ → current (code.if_then_else p s t c₀ c₁)
+  | if_then_else_right : ∀ p t pa pb q s (c₀ : code pa q) (c₁ : code pb q),
+         current c₁ → current (code.if_then_else p s t c₀ c₁)
+  | while_cond : ∀ p inv q s w (c : code p inv),
+         current (code.while q s w c)
+  | while_body : ∀ p inv q s w (c : code p inv),
+         current c → current (code.while q s w c)
 
 @[reducible]
 def seq_left {p q r} {c₀ : code p q} (c₁ : code q r)
@@ -63,54 +63,56 @@ def seq_right {p q r} (c₀ : code p q) {c₁ : code q r}
 current.seq_right _ _ _ c₀ _ cur
 
 @[reducible]
-def ite_cond (p t) {pa pb q} (c₀ : code pa q) (c₁ : code pb q)
-: current (if_then_else p t c₀ c₁) :=
-current.if_then_else_cond p t _ _ _ c₀ c₁
+def ite_cond (p t) {pa pb q} (s : set lbl) (c₀ : code pa q) (c₁ : code pb q)
+: current (if_then_else p s t c₀ c₁) :=
+current.if_then_else_cond p t _ _ _ s c₀ c₁
 
 @[reducible]
-def ite_left (p t) {pa pb q} {c₀ : code pa q} (c₁ : code pb q) (cur₀ : current c₀)
-: current (if_then_else p t c₀ c₁) :=
-current.if_then_else_left p t _ _ _ c₀ c₁ cur₀
+def ite_left (p t) {pa pb q} (s : set lbl) {c₀ : code pa q} (c₁ : code pb q) (cur₀ : current c₀)
+: current (if_then_else p s t c₀ c₁) :=
+current.if_then_else_left p t _ _ _ s c₀ c₁ cur₀
 
 @[reducible]
-def ite_right (p t) {pa pb q} (c₀ : code pa q) {c₁ : code pb q} (cur₁ : current c₁)
-: current (if_then_else p t c₀ c₁) :=
-current.if_then_else_right p t _ _ _ c₀ c₁ cur₁
+def ite_right (p t : pred) {pa pb q : pred} (s : set lbl)
+  (c₀ : code pa q) {c₁ : code pb q}
+  (cur₁ : current c₁)
+: current (if_then_else p s t c₀ c₁) :=
+current.if_then_else_right p t _ _ _ s c₀ c₁ cur₁
 
 @[reducible]
-def while_cond {p inv} (q w) (c : code p inv)
-: current (code.while q w c) :=
-current.while_cond p inv q w c
+def while_cond {p inv} (q s w) (c : code p inv)
+: current (code.while q s w c) :=
+current.while_cond p inv q s w c
 
 @[reducible]
-def while_body {p inv} (q w) {c : code p inv}
+def while_body {p inv} (q s w) {c : code p inv}
   (cur : current c)
-: current (code.while q w c) :=
-current.while_body p inv q w c cur
+: current (code.while q s w c) :=
+current.while_body p inv q s w c cur
 
 def selects' : Π {p q} {c : code p q}, current c → lbl → Prop
-  | ._ ._ ._ (current.action _ _ e') e := e = e'
+  | ._ ._ ._ (current.action _ _ _ e') e := e = e'
   | ._ ._ ._ (current.seq_left _ _ _ s c p) e := selects' p e
   | ._ ._ ._ (current.seq_right _ _ _ _ _ p) e := selects' p e
-  | ._ ._ ._ (current.if_then_else_cond _ _ _ _ _ _ _) e    := false
-  | ._ ._ ._ (current.if_then_else_left _ _ _ _ _ _ _ p) e  := selects' p e
-  | ._ ._ ._ (current.if_then_else_right _ _ _ _ _ _ _ p) e := selects' p e
-  | ._ ._ ._ (current.while_cond _ _ _ _ _) e   := false
-  | .(inv) .(q) ._ (current.while_body p inv q _ _ pc) e := selects' pc e
+  | ._ ._ ._ (current.if_then_else_cond _ _ _ _ _ _ _ _) e    := false
+  | ._ ._ ._ (current.if_then_else_left _ _ _ _ _ _ _ _ p) e  := selects' p e
+  | ._ ._ ._ (current.if_then_else_right _ _ _ _ _ _ _ _ p) e := selects' p e
+  | ._ ._ ._ (current.while_cond _ _ _ _ _ _) e   := false
+  | .(inv) .(q) ._ (current.while_body p inv q _ _ _ pc) e := selects' pc e
 
 def selects {p q} {c : code p q} : option (current c) → lbl → Prop
   | (some c) := selects' c
   | none := False
 
 def is_control' : Π {p q} {c : code p q}, current c → bool
-  | ._ ._ ._ (current.action _ _ l) := ff
+  | ._ ._ ._ (current.action _ _ _ l) := ff
   | ._ ._ ._ (current.seq_left  p q r _ _ pc)       := is_control' pc
   | ._ ._ ._ (current.seq_right p q r _ _ pc)       := is_control' pc
-  | .(p) .(q) ._ (current.if_then_else_cond  p t pa pb q _ _) := tt
-  | ._ ._ ._ (current.if_then_else_left  p t _ _ _ _ _ pc)    := is_control' pc
-  | ._ ._ ._ (current.if_then_else_right p t _ _ _ _ _ pc)    := is_control' pc
-  | .(inv) .(q) ._ (current.while_cond p inv q t _) := tt
-  | ._ ._ ._ (current.while_body _ _ _ _ _ pc)      := is_control' pc
+  | .(p) .(q) ._ (current.if_then_else_cond  p t pa pb q _ _ _) := tt
+  | ._ ._ ._ (current.if_then_else_left  p t _ _ _ _ _ _ pc)    := is_control' pc
+  | ._ ._ ._ (current.if_then_else_right p t _ _ _ _ _ _ pc)    := is_control' pc
+  | .(inv) .(q) ._ (current.while_cond p inv q _ t _) := tt
+  | ._ ._ ._ (current.while_body _ _ _ _ _ _ pc)      := is_control' pc
 
 def is_control {p q} {c : code p q} : option (current c) → bool
   | (some pc) := is_control' pc
@@ -130,14 +132,14 @@ def is_control {p q} {c : code p q} : option (current c) → bool
 --   | ._ ._ ._ (current.while_body p t inv q c cur) := is_control_decidable cur
 
 def condition' : Π {p q} {c : code p q} (pc : current c), is_control' pc → σ → Prop
-  | ._ ._ ._ (current.action _ _ _) h := by cases h
+  | ._ ._ ._ (current.action _ _ _ _) h := by cases h
   | ._ ._ ._ (current.seq_left  p q r c₀ c₁ pc) h := condition' pc h
   | ._ ._ ._ (current.seq_right p q r c₀ c₁ pc) h := condition' pc h
-  | .(p) .(q) ._ (current.if_then_else_cond  p c pa pb q c₀ c₁) h := c
-  | .(p) .(q) ._ (current.if_then_else_left  p c pa pb q c₀ c₁ pc) h := condition' pc h
-  | .(p) .(q) ._ (current.if_then_else_right p c pa pb q c₀ c₁ pc) h := condition' pc h
-  | .(inv) .(q) ._ (current.while_cond p inv q c _) h    := c
-  | .(inv) .(q) ._ (current.while_body p inv q _ _ pc) h := condition' pc h
+  | .(p) .(q) ._ (current.if_then_else_cond  p c pa pb q _ c₀ c₁) h := c
+  | .(p) .(q) ._ (current.if_then_else_left  p c pa pb q _ c₀ c₁ pc) h := condition' pc h
+  | .(p) .(q) ._ (current.if_then_else_right p c pa pb q _ c₀ c₁ pc) h := condition' pc h
+  | .(inv) .(q) ._ (current.while_cond p inv q _ c _) h    := c
+  | .(inv) .(q) ._ (current.while_body p inv q _ _ _ pc) h := condition' pc h
 
 def condition {p q} {c : code p q} : ∀ pc : option $ current c, is_control pc → σ → Prop
   | (some pc) := condition' pc
@@ -145,24 +147,24 @@ def condition {p q} {c : code p q} : ∀ pc : option $ current c, is_control pc 
 
 def action_of : Π {p q} {c : code p q} (cur : current c),
 { p // ∃ P, condition (some cur) P = p }  ⊕ subtype (selects (some cur))
-  | ._ ._ ._ (current.action _ _ l) := sum.inr ⟨l,rfl⟩
+  | ._ ._ ._ (current.action _ _ _ l) := sum.inr ⟨l,rfl⟩
   | ._ ._ ._ (current.seq_left  p q r _ _ pc) := action_of pc
   | ._ ._ ._ (current.seq_right p q r _ _ pc) := action_of pc
-  | .(p) .(q) ._ (current.if_then_else_cond  p t pa pb q _ _) := sum.inl ⟨t,rfl,rfl⟩
-  | ._ ._ ._ (current.if_then_else_left  p t _ _ _ _ _ pc) := action_of pc
-  | ._ ._ ._ (current.if_then_else_right p t _ _ _ _ _ pc) := action_of pc
-  | .(inv) .(q) ._ (current.while_cond p inv q t _)    := sum.inl ⟨t,rfl,rfl⟩
-  | ._ ._ ._ (current.while_body _ _ _ _ _ pc) := action_of pc
+  | .(p) .(q) ._ (current.if_then_else_cond  p t pa pb q _ _ _) := sum.inl ⟨t,rfl,rfl⟩
+  | ._ ._ ._ (current.if_then_else_left  p t _ _ _ _ _ _ pc) := action_of pc
+  | ._ ._ ._ (current.if_then_else_right p t _ _ _ _ _ _ pc) := action_of pc
+  | .(inv) .(q) ._ (current.while_cond p inv q _ t _)    := sum.inl ⟨t,rfl,rfl⟩
+  | ._ ._ ._ (current.while_body _ _ _ _ _ _ pc) := action_of pc
 
 def assert_of' : Π {p q} {c : code p q}, current c → σ → Prop
-  | .(p) ._ ._ (current.action p _ _) := p
+  | .(p) ._ ._ (current.action p _ _ _) := p
   | ._ ._ ._ (current.seq_left  _ _ _ _ _ pc) := assert_of' pc
   | ._ ._ ._ (current.seq_right _ _ _ _ _ pc) := assert_of' pc
-  | .(p) ._ ._ (current.if_then_else_cond  p _ _ _ _ _ _)  := p
-  | ._ ._ ._ (current.if_then_else_left  _ _ _ _ _ _ _ pc) := assert_of' pc
-  | ._ ._ ._ (current.if_then_else_right _ _ _ _ _ _ _ pc) := assert_of' pc
-  | .(inv) .(q) ._ (current.while_cond p inv q _ _)  := inv
-  | ._ ._ ._ (current.while_body _ _ _ _ _ pc) := assert_of' pc
+  | .(p) ._ ._ (current.if_then_else_cond  p _ _ _ _ _ _ _)  := p
+  | ._ ._ ._ (current.if_then_else_left  _ _ _ _ _ _ _ _ pc) := assert_of' pc
+  | ._ ._ ._ (current.if_then_else_right _ _ _ _ _ _ _ _ pc) := assert_of' pc
+  | .(inv) .(q) ._ (current.while_cond p inv q _ _ _)  := inv
+  | ._ ._ ._ (current.while_body _ _ _ _ _ _ pc) := assert_of' pc
 
 def assert_of {p q} {c : code p q} : option (current c) → σ → Prop
   | none := q
@@ -171,14 +173,14 @@ def assert_of {p q} {c : code p q} : option (current c) → σ → Prop
 local attribute [instance] classical.prop_decidable
 
 noncomputable def next_assert' : Π {p q} {c : code p q}, current c → σ → σ → Prop
-  | ._ .(q) ._ (current.action _ q _) := λ _, q
+  | ._ .(q) ._ (current.action _ q _ _) := λ _, q
   | ._ ._ ._ (current.seq_left  _ _ _ _ _ pc) := next_assert' pc
   | ._ ._ ._ (current.seq_right _ _ _ _ _ pc) := next_assert' pc
-  | .(p) .(q) ._ (current.if_then_else_cond  p t pa pb q _ _)  := λ s, if t s then pa else pb
-  | ._ ._ ._ (current.if_then_else_left  _ _ _ _ _ _ _ pc) := next_assert' pc
-  | ._ ._ ._ (current.if_then_else_right _ _ _ _ _ _ _ pc) := next_assert' pc
-  | .(inv) .(q) ._ (current.while_cond p inv q t _)  := λ s, if t s then p else q
-  | ._ ._ ._ (current.while_body _ _ _ _ _ pc) := next_assert' pc
+  | .(p) .(q) ._ (current.if_then_else_cond  p t pa pb q _ _ _)  := λ s, if t s then pa else pb
+  | ._ ._ ._ (current.if_then_else_left  _ _ _ _ _ _ _ _ pc) := next_assert' pc
+  | ._ ._ ._ (current.if_then_else_right _ _ _ _ _ _ _ _ pc) := next_assert' pc
+  | .(inv) .(q) ._ (current.while_cond p inv q _ t _)  := λ s, if t s then p else q
+  | ._ ._ ._ (current.while_body _ _ _ _ _ _ pc) := next_assert' pc
 
 noncomputable def next_assert {p q} {c : code p q} : option (current c) → σ → σ → Prop
   | none := λ _, q
@@ -186,37 +188,37 @@ noncomputable def next_assert {p q} {c : code p q} : option (current c) → σ �
 
 def first : Π {p q} (c : code p q), option (current c)
   | ._ ._ (code.skip p) := none
-  | ._ ._ (code.action p _ l) := some $ current.action _ _ _
+  | ._ ._ (code.action p _ _ l) := some $ current.action _ _ _ _
   | .(p) .(r) (@code.seq ._ ._ p q r c₀ c₁) :=
         seq_left c₁ <$> first _
     <|> seq_right _ <$> first _
-  | ._ ._ (@if_then_else ._ ._ p _ _ _ c b₀ b₁) :=
-    some $ ite_cond _ _ _ _
-  | ._ ._ (@code.while ._ ._ _ _ _ c b) :=
-    some $ while_cond _ _ _
+  | ._ ._ (@if_then_else ._ ._ p _ _ _ _ c b₀ b₁) :=
+    some $ ite_cond _ _ _ _ _
+  | ._ ._ (@code.while ._ ._ _ _ _ _ c b) :=
+    some $ while_cond _ _ _ _
 
 noncomputable def next' (s : σ) : ∀ {p q} {c : code p q}, current c → option (current c)
-  | ._ ._ ._ (current.action p q l) := none
+  | ._ ._ ._ (current.action p q _ l) := none
   | ._ ._ ._ (current.seq_left _ _ _ c₀ c₁ cur₀) :=
         seq_left c₁ <$> next' cur₀
     <|> seq_right c₀ <$> first c₁
   | ._ ._ ._ (current.seq_right _ _ _ c₀ c₁ cur₁) :=
         seq_right _ <$> next' cur₁
-  | .(p) .(q) ._ (current.if_then_else_cond p c pa pb q b₀ b₁) :=
+  | .(p) .(q) ._ (current.if_then_else_cond p c pa pb q _ b₀ b₁) :=
       if c s
-         then ite_left _ _ _ <$> first b₀
-         else ite_right _ _ _ <$> first b₁
-  | ._ ._ ._ (current.if_then_else_left _ _ _ _ _ b₀ b₁ cur₀) :=
-      ite_left _ _ b₁ <$> next' cur₀
-  | ._ ._ ._ (current.if_then_else_right _ _ _ _ _ b₀ b₁ cur₁) :=
-      ite_right _ _ _ <$> next' cur₁
-  | .(inv) .(q) ._ (current.while_cond p inv q c b) :=
+         then ite_left _ _ _ _ <$> first b₀
+         else ite_right _ _ _ _ <$> first b₁
+  | ._ ._ ._ (current.if_then_else_left _ _ _ _ _ _ b₀ b₁ cur₀) :=
+      ite_left _ _ _ b₁ <$> next' cur₀
+  | ._ ._ ._ (current.if_then_else_right _ _ _ _ _ _ b₀ b₁ cur₁) :=
+      ite_right _ _ _ _ <$> next' cur₁
+  | .(inv) .(q) ._ (current.while_cond p inv q ds c b) :=
       if c s
-      then while_body q c <$> first b <|> some (while_cond _ _ b)
+      then while_body q ds c <$> first b <|> some (while_cond _ ds _ b)
       else none
-  | ._ ._ ._ (current.while_body _ _ q c b cur) :=
-          while_body q c <$> next' cur
-      <|> some (while_cond _ _ b)
+  | ._ ._ ._ (current.while_body _ _ q _ c b cur) :=
+          while_body q _ c <$> next' cur
+      <|> some (while_cond _ _ _ b)
 
 noncomputable def next (s : σ) {p q : pred} {c : code p q}
 : option (current c) → option (current c)
